proof/crefine/Finalise_C.thy
@@ -16,7 +16,7 @@ context kernel_m
 begin
 
 lemma switchIfRequiredTo_ccorres [corres]:
-  "ccorres dc xfdc (valid_queues and valid_objs' and tcb_at' thread
+  "ccorres dc xfdc (valid_queues and valid_objs' and tcb_at' thread  and (\<lambda>s. ksCurDomain s \<le> maxDomain)
                           and (\<lambda>s. weak_sch_act_wf (ksSchedulerAction s) s) and st_tcb_at' runnable' thread)
                    (UNIV \<inter> \<lbrace>\<acute>target = tcb_ptr_to_ctcb_ptr thread\<rbrace>) hs
            (switchIfRequiredTo thread)
